Final cleanup of repo before submission.

rust.v
@@ -1,4 +1,5 @@
 Require Import Coq.ZArith.ZArith.
+Require Import Coq.Arith.EqNat.
 Require Import Coq.Lists.List.
 Require Import Lia.
 
@@ -15,9 +16,8 @@ match loc with
   | InvalidMem => None
 end.
 
-
 Inductive ref_type : Type :=
-| RefMut : mem_loc -> ref_type  
+| RefMut : mem_loc -> ref_type
 | RefImm : list mem_loc -> ref_type.
 
 Definition ref_to_mem_loc (ref : ref_type) : mem_loc :=
@@ -34,8 +34,9 @@ end.
 Inductive value : Type :=
 | VUnit : value
 | VInt : Z -> value
-| VRefMut : ref_type -> value
-| VRefImmMut : ref_type -> value.
+| VRefImmMut : ref_type -> value
+| VRefMut : ref_type -> value.
+
 
 Inductive var : Type := 
 | Var : nat -> var. 
@@ -46,22 +47,24 @@ match v with
 end.
 
 Inductive expression : Type :=
-| EValue: value -> expression                   
-| EVar : var -> expression                            
-| EAssign : mem_loc -> expression -> expression        
-| EMutBorrow : mem_loc -> expression             
-| EImmBorrow : mem_loc -> expression             
-| EDeref : expression -> expression                
-| ELet : var -> expression -> expression -> expression
-| EMut : var -> expression -> expression
-| ESequence : expression -> expression -> expression.          
+| EValue: value -> expression (* 10; *)                  
+| EVar : var -> expression (* a; *)                           
+| EAssign : mem_loc -> expression -> expression (* a = 10; *)
+| EImmBorrow : mem_loc -> expression (* b = &a; *)  
+| EMutBorrow : mem_loc -> expression (* b = &a; *)               
+| EDeref : expression -> expression (* *a *)               
+| ELet : var -> expression -> expression -> expression (* let a = 10;a;*)
+| EMut : var -> expression -> expression (* let mut a = 10; *)
+| ESequence : expression -> expression -> expression.  (* let mut a 10; a = 5;*)       
 
 
 Inductive ownership : Type :=
 | Own : value -> ownership 
-| BorrowMut : mem_loc -> ownership               
+| OwnMut : value -> ownership
 | BorrowImm : list mem_loc -> ownership
-| OwnMut : value -> ownership.
+| BorrowMut : mem_loc ->  ownership.      
+
+
 
 Definition memory_state := 
 mem_loc -> option ownership.
@@ -78,9 +81,10 @@ Definition eqb_option_nat (o1 o2 : option nat) : bool :=
   | _, _ => false
   end.
   
-Definition update_memory (m : memory_state) (loc : mem_loc) (v : option ownership) : memory_state :=
- fun l =>
-    if eqb_option_nat (mem_loc_to_nat l) (mem_loc_to_nat loc) then v else m l.
+Definition update_memory (m : memory_state) (loc : mem_loc) (o : option ownership) : memory_state :=
+fun l => 
+    if eqb_option_nat (mem_loc_to_nat l) (mem_loc_to_nat loc) 
+    then o else m l.
 
 Inductive eval_result : Type :=
 | EvalSuccess : memory_state -> value -> eval_result
@@ -92,6 +96,13 @@ with eval_error : Type :=
 | TypeMismatch : eval_error
 | OtherError : eval_error.
 
+Inductive eval_result_2 : Type :=
+| EvalSuccess2 
+| EvalError2.
+
+
+
+
 Lemma success_neq_failure :
 forall (m : memory_state) (v : value) (err : eval_error ),
 EvalSuccess m v <> EvalError err.
@@ -101,72 +112,73 @@ intros. discriminate. Qed.
 
 Fixpoint eval (m : memory_state) (e : expression) : eval_result :=
 match e with
-  | EValue v => EvalSuccess m v
-  | EVar x =>
+| EValue v => EvalSuccess m v
+| EVar x =>
     match m (MemLoc (var_to_nat x)) with
     | Some (Own v) => EvalSuccess m v
     | Some (OwnMut v) => EvalSuccess m v
     | Some (BorrowMut loc) => EvalSuccess m (VRefMut (RefMut loc))
-    | Some (BorrowImm locs) => EvalSuccess m (VRefImmMut (RefImm (MemLoc (var_to_nat x) :: locs)))
+    | Some (BorrowImm locs) => EvalSuccess m (VRefImmMut (RefImm locs))
     | None => EvalError (UninitializedMemory (MemLoc (var_to_nat x)))
     end
-  | EAssign loc e' =>
-    match eval m e' with
-      | EvalSuccess m' v =>
-          match m loc with
-          | Some (OwnMut _) =>
-              EvalSuccess (update_memory m' loc (Some (OwnMut v))) v
-          | Some _ => EvalError (InvalidAssignment loc)
-          | None => EvalError (UninitializedMemory loc)
-          end
-      | EvalError err => EvalError err
+| EAssign loc e' =>
+  match eval m e' with
+  | EvalSuccess m' v =>
+      match m loc with
+      | Some (OwnMut _) =>
+          EvalSuccess (update_memory m' loc (Some (OwnMut v))) v
+      | Some _ => EvalError (InvalidAssignment loc)
+      | None => EvalError (UninitializedMemory loc)
+      end
+  | EvalError err => EvalError err
+  end
+| EImmBorrow loc =>
+  match m loc with
+  | Some (Own v) => EvalSuccess (update_memory m loc (Some (BorrowImm (loc :: nil)))) (VRefImmMut (RefImm (loc :: nil)))
+  | Some (BorrowImm l) => EvalSuccess (update_memory m loc (Some (BorrowImm (loc :: l)))) (VRefImmMut (RefImm (loc :: l)))
+  | Some _ => EvalError (BorrowConflict loc)
+  | None => EvalError (UninitializedMemory loc)
+  end
+| EMutBorrow loc =>
+    match m loc with
+    | Some (Own v) => EvalSuccess (update_memory m loc (Some (BorrowMut loc))) (VRefMut (RefMut loc))
+    | Some _ => EvalError (BorrowConflict loc)
+    | None => EvalError (UninitializedMemory loc)
     end
-  | EMut x e' =>
-      match eval m e' with
-      | EvalSuccess m' v =>
-          EvalSuccess (update_memory m' (MemLoc (var_to_nat x)) (Some (OwnMut v))) VUnit
-      | EvalError err => EvalError err
-      end
-  | EMutBorrow loc =>
-      match m loc with
-      | Some (Own v) => EvalSuccess (update_memory m loc (Some (BorrowMut loc))) (VRefMut (RefMut loc))
-      | Some _ => EvalError (BorrowConflict loc)
-      | None => EvalError (UninitializedMemory loc)
-      end
-  | EImmBorrow loc =>
-      match m loc with
-      | Some (Own v) => EvalSuccess (update_memory m loc (Some (BorrowImm (loc :: nil)))) (VRefImmMut (RefImm (loc :: nil)))
-      | Some (BorrowImm l) => EvalSuccess (update_memory m loc (Some (BorrowImm (loc :: l)))) (VRefImmMut (RefImm (loc :: l)))
-      | Some _ => EvalError (BorrowConflict loc)
-      | None => EvalError (UninitializedMemory loc)
-      end
-  | EDeref e' =>
-      match eval m e' with
-      | EvalSuccess m' (VRefMut ref) =>
-          match m (ref_to_mem_loc ref) with
-          | Some (OwnMut v) => EvalSuccess m' v
-          | _ => EvalError (BorrowConflict (ref_to_mem_loc ref))
-          end
-      | EvalSuccess m' (VRefImmMut loc) =>
-          match m (ref_to_mem_loc loc) with
-          | Some (Own v) => EvalSuccess m' v
-          | _ => EvalError (BorrowConflict (ref_to_mem_loc loc))
-          end
-      | EvalSuccess _ _ => EvalError TypeMismatch
-      | EvalError err => EvalError err
-      end
-  | ELet x e1 e2 =>
-      match eval m e1 with
-      | EvalSuccess m' v =>
-          let new_m := update_memory m' (MemLoc (var_to_nat x)) (Some (Own v)) in
-          eval new_m e2
-      | EvalError err => EvalError err
-      end
-  | ESequence e1 e2 =>
-      match eval m e1 with
-      | EvalSuccess m' _ => eval m' e2
-      | EvalError err => EvalError err
-      end
+
+| EDeref e' =>
+    match eval m e' with
+    | EvalSuccess m' (VRefMut ref) =>
+        match m (ref_to_mem_loc ref) with
+        | Some (OwnMut v) => EvalSuccess m' v
+        | _ => EvalError (BorrowConflict (ref_to_mem_loc ref))
+        end
+    | EvalSuccess m' (VRefImmMut loc) =>
+        match m (ref_to_mem_loc loc) with
+        | Some (Own v) => EvalSuccess m' v
+        | _ => EvalError (BorrowConflict (ref_to_mem_loc loc))
+        end
+    | EvalSuccess _ _ => EvalError TypeMismatch
+    | EvalError err => EvalError err
+    end
+| ELet x e1 e2 =>
+    match eval m e1 with
+    | EvalSuccess m' v =>
+        let new_m := update_memory m' (MemLoc (var_to_nat x)) (Some (Own v)) in
+        eval new_m e2
+    | EvalError err => EvalError err
+    end
+| EMut x e' =>
+  match eval m e' with
+  | EvalSuccess m' v =>
+      EvalSuccess (update_memory m' (MemLoc (var_to_nat x)) (Some (OwnMut v))) VUnit
+  | EvalError err => EvalError err
+  end
+| ESequence e1 e2 =>
+    match eval m e1 with
+    | EvalSuccess m' _ => eval m' e2
+    | EvalError err => EvalError err
+    end
 end.
 
 
@@ -182,117 +194,123 @@ Qed.
 
 
 Inductive borrow_valid : memory_state -> mem_loc -> borrow_state -> Prop :=
-  | BorrowMutValid : forall m loc,
+  | BorrowMutValid : forall (m : memory_state) (loc : mem_loc),
       m loc = Some (BorrowMut loc) ->
       borrow_valid m loc (MutBorrowed loc)
-  | BorrowImmValid : forall m loc bs,
-      m loc = Some (BorrowImm bs) ->
-      Forall (fun r => m r = Some (BorrowImm bs)) bs ->
-      borrow_valid m loc (ImmBorrowed bs).
+  | BorrowImmValid : forall (m : memory_state) (loc : mem_loc) (locs : list mem_loc),
+      m loc = Some (BorrowImm locs) ->
+      Forall (fun l => m l = Some (BorrowImm locs)) locs ->
+      borrow_valid m loc (ImmBorrowed locs).
 
 
 Inductive well_typed : lifetime_state -> memory_state -> expression -> ref_type -> Prop :=
-| TValInt : forall (l : lifetime_state) (m : memory_state) (z : Z),
-    well_typed l m (EValue (VInt z)) (RefImm (MemLoc 0 :: nil)) 
-
-| TValRefMut : forall (l : lifetime_state) (m : memory_state) (loc : mem_loc),
-    well_typed l m (EValue (VRefMut (RefMut loc))) (RefMut loc) 
-
-| TValRefImm : forall (l : lifetime_state) (m : memory_state) (loc : mem_loc),
-    well_typed l m (EValue (VRefImmMut (RefImm (loc :: nil)))) (RefImm (loc :: nil)) 
 
 | TValUnit : forall (l : lifetime_state) (m : memory_state),
-    well_typed l m (EValue VUnit) (RefImm (MemLoc 0 :: nil))
+  eval m (EValue (VUnit)) = EvalSuccess m (VUnit) ->
+  well_typed l m (EValue VUnit) (RefImm (MemLoc 0 :: nil))
+| TValInt : forall (l : lifetime_state) (m : memory_state) (z : Z),
+  eval m (EValue (VInt z)) = EvalSuccess m (VInt z) ->
+  well_typed l m (EValue (VInt z)) (RefImm (MemLoc 0 :: nil)) 
+
+| TValRefImm : forall (l : lifetime_state) (m : memory_state) (locs : list mem_loc),
+  eval m (EValue (VRefImmMut (RefImm (locs)))) = EvalSuccess m (VRefImmMut (RefImm (locs))) ->
+  well_typed l m (EValue (VRefImmMut (RefImm (locs)))) (RefImm (locs)) 
+| TValRefMut : forall (l : lifetime_state) (m : memory_state) (loc : mem_loc),
+  eval m (EValue (VRefMut (RefMut loc))) = EvalSuccess m (VRefMut (RefMut loc)) ->
+  well_typed l m (EValue (VRefMut (RefMut loc))) (RefMut loc) 
 
 | TVar : forall (l : lifetime_state) (m : memory_state) (x : var) (r : ref_type),
+    eval m (EVar x) = 
     match m (MemLoc (var_to_nat x)) with
-    | Some (Own _) => r = RefImm (MemLoc (var_to_nat x) :: nil)
-    | Some (BorrowMut loc) => r = RefMut loc
-    | Some (BorrowImm locs) => r = RefImm (MemLoc (var_to_nat x) :: locs)
-    | _ => False 
+    | Some (Own _) => EvalSuccess m (VRefImmMut ( RefImm (MemLoc (var_to_nat x) :: nil)))
+    | Some (OwnMut _) => EvalSuccess m (VRefMut ( RefMut (MemLoc (var_to_nat x))))
+    | Some (BorrowImm locs) => EvalSuccess m (VRefImmMut (RefImm (locs)))
+    | Some (BorrowMut loc) => EvalSuccess m (VRefMut (RefMut loc ))
+    | None => EvalError (UninitializedMemory (MemLoc (var_to_nat x)))
     end ->
     well_typed l m (EVar x) r
+| TAssign : forall (l : lifetime_state) (m : memory_state) (loc : mem_loc) (e : expression),
+    well_typed l m e (RefMut loc) ->
+    well_typed l m (EAssign loc e) (RefMut loc)
+| TImmBorrow : forall (l : lifetime_state) (m : memory_state) (x : var) (locs : list mem_loc),
+    well_typed l m (EVar x) (RefImm (locs))->
+    well_typed l m (EImmBorrow (MemLoc (var_to_nat x))) (RefImm (locs))
 | TMutBorrow : forall (l : lifetime_state) (m : memory_state) (x : var) (loc : mem_loc),
     well_typed l m (EVar x) (RefMut loc) ->
     well_typed l m (EMutBorrow (MemLoc (var_to_nat x))) (RefMut loc)
-
-| TImmBorrow : forall (l : lifetime_state) (m : memory_state) (x : var) (loc : mem_loc),
-    well_typed l m (EVar x) (RefImm (loc :: nil))->
-    well_typed l m (EImmBorrow (MemLoc (var_to_nat x))) (RefImm (loc :: nil))
-
+| TDerefImm : forall (l : lifetime_state) (m : memory_state) (e: expression) (loc : list mem_loc),
+    well_typed l m e (RefImm loc) ->
+    well_typed l m (EDeref e) (RefImm loc)
+| TDerefMut : forall (l : lifetime_state) (m : memory_state) (e : expression) (loc : mem_loc),
+    well_typed l m e (RefMut loc) ->
+    well_typed l m (EDeref e) (RefMut loc)
+| TLet : forall (l : lifetime_state) (m : memory_state) (x : var) (e1 e2 : expression) (r1 r2 : ref_type),
+    well_typed l m e1 r1 ->
+    well_typed l (update_memory m (MemLoc (var_to_nat x)) (Some (Own (VInt 0)))) e2 r2 ->
+    well_typed l m (ELet x e1 e2) r2
 | TMut : forall (l : lifetime_state) (m : memory_state) (x : var) (e : expression) (r : ref_type),
     well_typed l m e r ->
-    well_typed l m (EMut x e) r.
+    well_typed l m (EMut x e) r
+| TSequence : forall (l : lifetime_state) (m : memory_state) (e1 e2 : expression) (r : ref_type),
+    well_typed l m e1 r ->
+    well_typed l m e2 r ->
+    well_typed l m (ESequence e1 e2) r.
 
-(* Theorem type_safety : 
-forall (l : lifetime_state) (m : memory_state) (e : expression) (r : ref_type) (m' : memory_state) (v : value) (err : eval_error),
- well_typed l m e r ->             
-  (exists m' v, eval m e = EvalSuccess m' v) \/ eval m e = EvalError err.
+Lemma eval_value :
+  forall (l : lifetime_state) (m : memory_state) (v : value) (r : ref_type),
+  well_typed l m (EValue v) r ->
+  exists m' v', eval m (EValue v) = EvalSuccess m' v'.
 Proof.
-  (* intros l m e r Htype. *)
-  intros l m e r m' v err Htype.
-  generalize dependent v.
-  induction e.
-  - left. exists m, v. simpl. reflexivity.
-  - simpl. destruct (m (MemLoc (var_to_nat v))).
-    + destruct o.
-      * left. exists m, v0. reflexivity.
-      * right. reflexivity.
-      * right. reflexivity.
-      * left. exists m, v0. reflexivity.
-    + right. reflexivity.
-  - intros v. inversion Htype.
-  - simpl. inversion Htype. subst r. rewrite <- H in *.  destruct (m (MemLoc (var_to_nat x))) eqn:Hlookup.
-    + destruct o.
-      * left. 
-      exists (update_memory m (MemLoc (var_to_nat x)) (Some (BorrowMut (MemLoc (var_to_nat x))))),
-      (VRefMut (RefMut (MemLoc (var_to_nat x)))).
-reflexivity.
-      * right. reflexivity.
-      * right. reflexivity.
-      * right. reflexivity.
-    + right. reflexivity.
-  - simpl. inversion Htype. subst r. rewrite <- H in *. destruct (m (MemLoc (var_to_nat x))).
-    + destruct o.
-      * left. exists (update_memory m (MemLoc (var_to_nat x)) (Some (BorrowImm (MemLoc (var_to_nat x) :: nil)))).
-      exists (VRefImmMut (RefImm (MemLoc (var_to_nat x)))). reflexivity.
-      * right. reflexivity.
-      * left. exists (update_memory m (MemLoc (var_to_nat x)) (Some (BorrowImm (MemLoc (var_to_nat x) :: l1)))).
-      exists (VRefImmMut (RefImm (MemLoc (var_to_nat x)))). reflexivity.
-      * right. reflexivity.
-    + right. reflexivity.
-  - inversion Htype.
-  - inversion Htype.
-  - intros. simpl. inversion Htype.
-    destruct (IHe H4) as [[m'' [v' Heval]] | Heval].
-    + auto.
-    + simpl.
-      destruct (m (MemLoc (var_to_nat v))) eqn:Hlookup.
-      * (* Case: m (MemLoc (var_to_nat v)) = Some _ *)
-        (* right. reflexivity. Borrow fails because the location is already in use *)
-      (* * Case: m (MemLoc (var_to_nat v)) = None *)
-      (* * destruct v'.
-        -- (* Case: v' = VInt z *)
-          exists (update_memory m'' (MemLoc (var_to_nat v)) (Some (OwnMut (VInt 0)))).
-          exists VUnit.
-          reflexivity.
-        * (* Case: v' = VRefMut loc *)
-          right. reflexivity. (* Borrow fails for invalid value *)
-        * (* Case: v' = VRefImm loc *)
-          right. reflexivity. (* Borrow fails for invalid value *)
-        * (* Case: v' = VUnit *)
-          right. reflexivity. (* Borrow fails for invalid value *)
-        reflexivity. *)
-Admitted. *)
-
-Lemma none_some_neq : forall (m : memory_state) (v : value), None <> Some (m, v).
-Proof.
-  intros m v H.
-  discriminate H.
+  intros l m v r H.
+  destruct v; try (exists m, v; reflexivity).
+  - (* VUnit *)
+    exists m, VUnit. reflexivity.
+  - (* VInt z *)
+    exists m, (VInt z). reflexivity.
+  - (* VRefImmMut ref *) 
+    exists m, (VRefImmMut (r0)). reflexivity.
+  - (* VRefImmMut ref *)
+    exists m, (VRefMut (r0)). reflexivity.
 Qed.
 
+Lemma eval_var :
+  forall (l : lifetime_state) (m : memory_state) (x : var) (r : ref_type),
+  well_typed l m (EVar x) r ->
+  exists v', eval m (EVar x) = EvalSuccess m v'.
+Proof.
+  intros l m x r H.
+  destruct (m (MemLoc (var_to_nat x))); try (exists m, VUnit; reflexivity).
+  - destruct o as [own | ownmut | borrowimm locs | borrowmut loc ]; try (exists m, VUnit; reflexivity).
+  + (* Some (Own v) *) destruct own.
+    --  simpl. inversion H. subst.  exists VUnit. admit.
+    -- admit. (* Some (OwnMut v) *)
+    -- admit.
+    -- admit.
+    + admit.
+  Admitted.
 
-Theorem type_safety_2 : 
+Lemma eval_assign :
+  forall (l : lifetime_state) (m : memory_state) (loc : mem_loc) (e : expression) (r : ref_type),
+  well_typed l m (EAssign loc e) r ->
+  exists m' v', eval m (EAssign loc e) = EvalSuccess m' v'.
+Proof.
+  intros l m loc e r H.
+
+Admitted.
+
+(* Theorem type_safety : 
+forall (l : lifetime_state) (m : memory_state) (e : expression) (r : ref_type) (m' : memory_state) (v : value),
+ well_typed l m e r ->             
+  (exists m' v, eval m e = EvalSuccess m' v).
+Proof.
+    intros l m e r H.
+     induction e; intros; try (apply eval_value in H0; assumption).
+  - apply eval_var in H0. exists m. assumption.
+  -  apply eval_assign in H0. assumption.
+  - ass
+   *)
+
+Theorem type_safety : 
 forall (l : lifetime_state) (m : memory_state) (e : expression) (r : ref_type) (m' : memory_state) (v : value),
  well_typed l m e r ->             
   (exists m' v, eval m e = EvalSuccess m' v).
@@ -300,41 +318,42 @@ Proof.
   intros l m e r m' v Htype.
   induction Htype.
 
+  (* Case: TValUnit *)
+  - exists m, VUnit. reflexivity.
+
   (* Case: TValInt *)
   - exists m, (VInt z). reflexivity.
 
+  (* Case: TValRefImm *)
+  - exists m, (VRefImmMut (RefImm (locs))). reflexivity.
+
   (* Case: TValRefMut *)
   - exists m, (VRefMut (RefMut loc)). reflexivity.
-
-  (* Case: TValRefImm *)
-  - exists m, (VRefImmMut (RefImm (loc :: nil))). reflexivity.
-
-  (* Case: TValUnit *)
-  - exists m, VUnit. reflexivity.
 
   (* Case: TVar (EVar x) *)
   - intros. simpl. destruct (m (MemLoc (var_to_nat x))) eqn:Hmem.
     + destruct o.
       * exists m, v0. reflexivity.
+      * exists m, v0. reflexivity.
+      * exists m, (VRefImmMut (RefImm (l0))). reflexivity.
       * exists m, (VRefMut (RefMut m0)). reflexivity. (* apply none_some_neq with (m := m) (v := v). *)
-      * exists m, (VRefImmMut (RefImm (MemLoc (var_to_nat x) :: l0))). reflexivity.
-        (* exfalso. assumption. *)
-      * exfalso. assumption. 
-    + exfalso. assumption. 
+    (* exfalso. assumption. *)
+    +  destruct (m (MemLoc (var_to_nat x))) eqn:Hmem2.
+    * (* Case: m (MemLoc (var_to_nat x)) = Some o *) discriminate Hmem.  (* Analyze valid memory states *)
+    * exists m, v. simpl in H. rewrite Hmem2 in H. exfalso.
+    apply success_neq_failure with
+    (err := UninitializedMemory (MemLoc (var_to_nat x)))
+    (m := m') (v := v). 
+    assert (EvalError (UninitializedMemory (MemLoc (var_to_nat x))) <> EvalSuccess m' v).
+      {
+        (* Step 3: Use distinctness of constructors *)
+        intros Hcontra. discriminate Hcontra. (* EvalError and EvalSuccess are distinct *)
+      }
+    admit.
+    
 
-  (* Case: TMutBorrow *)
-  - destruct (m (MemLoc (var_to_nat x))) eqn:Hmem.
-    + destruct o.
-      * exists (update_memory m (MemLoc (var_to_nat x)) (Some (BorrowMut (MemLoc (var_to_nat x))))),
-               (VRefMut (RefMut (MemLoc (var_to_nat x)))).
-        simpl. rewrite Hmem. reflexivity.
-      * simpl in *. rewrite Hmem in *.  destruct IHHtype. destruct H. injection H. exists m, v. admit.
-      * simpl in *. rewrite Hmem in *. absurd (EvalSuccess m v = EvalError (BorrowConflict (MemLoc (var_to_nat x)))). 
-        -- discriminate.
-        -- destruct IHHtype. destruct H. admit.
-      * exists (update_memory m (MemLoc (var_to_nat x)) (Some (BorrowMut (MemLoc (var_to_nat x))))),
-               (VRefMut (RefMut (MemLoc (var_to_nat x)))). simpl. admit.
-    +  exists m, v. simpl. rewrite Hmem. admit.
+  - admit.
+  
 
   (* Case: TImmBorrow (EImmBorrow) *)
   - destruct (m (MemLoc (var_to_nat x))) eqn:Hmem.
@@ -358,12 +377,27 @@ Proof.
                                 (Some (BorrowMut (MemLoc (var_to_nat x))))),
                 (VRefImmMut (RefImm (MemLoc (var_to_nat x) :: nil))).
       simpl. rewrite Hmem. admit.
-
- (* Case: TMut *)
-- simpl. 
-  destruct IHHtype as [m'' [v' Heval]].
-  exists (update_memory m'' (MemLoc (var_to_nat x)) (Some (OwnMut v'))), VUnit. 
-
+  (* Case: TMutBorrow *)
+  - destruct (m (MemLoc (var_to_nat x))) eqn:Hmem.
+    + destruct o.
+      * exists (update_memory m (MemLoc (var_to_nat x)) (Some (BorrowMut (MemLoc (var_to_nat x))))),
+               (VRefMut (RefMut (MemLoc (var_to_nat x)))).
+        simpl. rewrite Hmem. reflexivity.
+      * simpl in *. rewrite Hmem in *.  destruct IHHtype. destruct H. injection H. exists m, v. admit.
+      * simpl in *. rewrite Hmem in *. absurd (EvalSuccess m v = EvalError (BorrowConflict (MemLoc (var_to_nat x)))). 
+        -- discriminate.
+        -- destruct IHHtype. destruct H. admit.
+      * exists (update_memory m (MemLoc (var_to_nat x)) (Some (BorrowMut (MemLoc (var_to_nat x))))),
+               (VRefMut (RefMut (MemLoc (var_to_nat x)))). simpl. admit.
+    +  exists m, v. simpl. rewrite Hmem. admit.
+  - (* Case: TDerefImm *) admit.
+  - (* Case: TDerefMut*) admit.
+  - (* Case: TLet*) admit.
+  - (* Case: TMut*)simpl. 
+    destruct IHHtype as [m'' [v' Heval]].
+    exists (update_memory m'' (MemLoc (var_to_nat x)) (Some (OwnMut v'))), VUnit.  admit.
+  - (* Case: TSeq*)admit.
+  (* Case: TMut *)
 Admitted.
 
 
@@ -375,6 +409,7 @@ forall (l : lifetime_state) (m : memory_state) (e: expression) (r : ref_type) (m
   eval m e = EvalSuccess m' v -> 
   borrow_valid m' loc bs.
 Proof.
+  intros l m e r m' v loc bs HType.
 Admitted.
 
 
